
31.
$$
\int\left(a+bx\right)^{n}\mathrm{d}x=\dfrac{\left(a+bx\right)^{n+1}}{\left(n+1\right)b},\left(n\ne1\right) 
$$

32.
$$
\int x\left(a+bx\right)\mathrm{d}x=\dfrac{x^{2}}{2}\left(a+\dfrac{2b}{3}x\right) 
$$

33.
$$
\int x^{2}\left(a+bx\right)\mathrm{d}x=\dfrac{x^{3}}{3}\left(a+\dfrac{3b}{4}x\right) 
$$

34.
$$
\int x^{m}\left(a+bx\right)\mathrm{d}x=\dfrac{x^{m+1}}{m+1}\left(a+\dfrac{\left(m+1\right)b}{m+2}x\right),\left(m\ne1,-2\right) 
$$

35.
$$
\int x\left(a+bx\right)^{n}\mathrm{d}x=\dfrac{1}{b^{2}\left(n+2\right)}\left(a+bx\right)^{n+2}-\dfrac{a}{b^{2}\left(n+1\right)}\left(a+bx\right)^{n+1},\left(n\ne1,-2\right) 
$$

36.
$$
x^{2}\left(a+bx\right)^{n}\mathrm{d}x=\dfrac{1}{b^{3}}\left(\dfrac{\left(a+bx\right)^{n+3}}{n+3}-2a\dfrac{\left(a+bx\right)^{n+2}}{n+2}+a^{2}\dfrac{\left(a+bx\right)^{n+1}}{n+1}\right),\left(n\ne1,-2,-3\right) 
$$

37.
$$
\int x^{m}\left(a+bx\right)^{n}\mathrm{d}x=\dfrac{x^{m+1}\left(a+bx\right)^{n}}{m+n+1}+\dfrac{an}{m+n+1}\int x^{m}\left(a+bx\right)^{n-1}
    =\dfrac{1}{a\left(n+1\right)}\left(-x^{m+1}\left(a+bx\right)^{n+1}+\left(m+n+2\right)\int x^{m}\left(a+bx\right)^{n+1}\mathrm{d}x\right)
    =\dfrac{1}{b\left(m+n+1\right)}\left(x^{m}\left(a+bx\right)^{n+1}-ma\int x^{m-1}\left(a+bx\right)^{n}\mathrm{d}x\right)
$$

38.
$$
\int\dfrac{a+bx}{x}\mathrm{d}x=a\ln\left|x\right|+bx
$$

39.
$$
\int\dfrac{a+bx}{x^{2}}\mathrm{d}x=b\ln\left|x\right|-\dfrac{a}{x}
$$

40.
$$
\int\dfrac{a+bx}{x^{3}}\mathrm{d}x=-\dfrac{a}{2x^{2}}-\dfrac{b}{x}
$$

41.
$$
\int\dfrac{a+bx}{x^{n}}\mathrm{d}x=-\dfrac{a}{\left(n-1\right)x^{n-1}}-\dfrac{b}{\left(n-2\right)x^{n-2}},\left(n>2\right) 
$$

42.
$$
\int\dfrac{\mathrm{d}x}{a+bx}=\dfrac{1}{b}\ln\left|a+bx\right|
$$

43.
$$
\int\dfrac{\mathrm{d}x}{\left(a+bx\right)^{2}}=-\dfrac{1}{b\left(a+bx\right)}
$$

44.
$$
\int\dfrac{\mathrm{d}x}{\left(a+bx\right)^{3}}=-\dfrac{1}{2b\left(a+bx\right)^{2}}
$$

45.
$$
\int\dfrac{\mathrm{d}x}{\left(a+bx\right)^{4}}=-\dfrac{1}{3b\left(a+bx\right)^{3}}
$$

46.
$$
\int\dfrac{\mathrm{d}x}{\left(a+bx\right)^{5}}=-\dfrac{1}{4b\left(a+bx\right)^{4}}
$$

47.
$$
\int\dfrac{\mathrm{d}x}{\left(a+bx\right)^{n}}=-\dfrac{1}{\left(n-1\right)b\left(a+bx\right)^{n-1}},\left(n\neq 0,1\right) 
$$

48.
$$
\int\dfrac{x}{a+bx}\mathrm{d}x=\dfrac{x}{b}-\dfrac{a}{b^{2}}\ln\left|a+bx\right|
$$

49.
$$
\int\dfrac{x}{\left(a+bx\right)^{2}}\mathrm{d}x=\dfrac{1}{b^{2}}\left(\ln\left|a+bx\right|+\dfrac{1}{a+bx}\right)
$$

50.
$$
\int\dfrac{x}{\left(a+bx\right)^{3}}\mathrm{d}x=-\dfrac{2\left(a+bx\right)-a}{2b^{2}\left(a+bx\right)^{2}}
$$

51.
$$
\int\dfrac{x}{\left(a+bx\right)^{4}}\mathrm{d}x=-\left(\dfrac{x}{2b}+\dfrac{a}{6b^{2}}\right)\dfrac{1}{\left(a+bx\right)^{3}}
$$

52.
$$
\int\dfrac{x}{\left(a+bx\right)^{5}}\mathrm{d}x=-\left(\dfrac{x}{3b}+\dfrac{a}{12b^{2}}\right)\dfrac{1}{\left(a+bx\right)^{4}}
$$

53.
$$
\int\dfrac{x}{\left(a+bx\right)^{n}}\mathrm{d}x=\dfrac{1}{b^{2}}\left(-\dfrac{1}{\left(n-2\right)\left(a+bx\right)^{n-2}}+\dfrac{a}{\left(n-1\right)\left(a+bx\right)^{n-1}}\right),\left(n\neq 1,2\right) 
$$

54.
$$
\int\dfrac{x^{2}}{a+bx}\mathrm{d}x=\dfrac{1}{b^{3}}\left(\dfrac{1}{2}\left(a+bx\right)^{2}-2a\left(a+bx\right)+a^{2}\ln\left|a+bx\right|\right) 
$$

55.
$$
\int\dfrac{x^{2}}{\left(a+bx\right)^{2}}\mathrm{d}x=\dfrac{1}{b^{3}}\left(a+bx-2a\ln\left|a+bx\right|-\dfrac{a^{2}}{a+bx}\right) 
$$

56.
$$
\int\dfrac{x^{2}}{a+bx}\mathrm{d}x=\dfrac{1}{b^{3}}\left(\dfrac{1}{2}\left(a+bx\right)^{2}-2a\left(a+bx\right)+a^{2}\ln\left|a+bx\right|\right) 
$$

57.
$$
\int\dfrac{x^{2}}{\left(a+bx\right)^{4}}\mathrm{d}x=-\left(\dfrac{x^{2}}{b}+\dfrac{ax}{b^{2}}+\dfrac{a^{2}}{3b^{3}}\right)\dfrac{1}{\left(a+bx\right)^{3}}
$$

58.
$$
\int\dfrac{x^{2}}{\left(a+bx\right)^{5}}\mathrm{d}x=-\left(\dfrac{x^{2}}{2b}+\dfrac{ax}{3b^{2}}+\dfrac{a^{2}}{12b^{3}}\right)\dfrac{1}{\left(a+bx\right)^{4}}
$$

59.
$$
\int\dfrac{x^{2}}{\left(a+bx\right)^{n}}\mathrm{d}x=\dfrac{1}{b^{3}}\left(-\dfrac{1}{\left(n-3\right)\left(a+bx\right)^{n-3}}+\dfrac{2a}{\left(n-2\right)\left(a+bx\right)^{n-2}}-\dfrac{a^{2}}{\left(n-1\right)\left(a+bx\right)^{n-1}}\right),\left(n\neq 1,2,3\right) 
$$

60.
$$
\int\dfrac{x^{3}}{a+bx}\mathrm{d}x=\dfrac{x^{3}}{3b}-\dfrac{ax^{2}}{2b^{2}}+\dfrac{a^{2}x}{b^{3}}-\dfrac{a^{3}}{b^{4}}\ln\left|a+bx\right|
$$

61.
$$
\int\dfrac{x^{3}}{\left(a+bx\right)^{2}}\mathrm{d}x=\left(\dfrac{x^{3}}{3b}-\dfrac{3ax^{2}}{2b^{2}}-\dfrac{2a^{2}x}{b^{3}}+\dfrac{a^{3}}{b^{4}}\right)\dfrac{1}{a+bx}+\dfrac{3a^{2}}{b^{4}}\ln\left|a+bx\right|
$$

62.
$$
\int\dfrac{x^{3}}{\left(a+bx\right)^{3}}\mathrm{d}x=\left(\dfrac{x}{b}+\dfrac{2ax^{2}}{b^{2}}-\dfrac{2a^{2}x}{b^{3}}-\dfrac{5a^{3}}{2b^{4}}\right)\dfrac{1}{\left(a+bx\right)^{2}}-\dfrac{3a}{b^{4}}\ln\left|a+bx\right|
$$

63.
$$
\int\dfrac{x^{3}}{\left(a+bx\right)^{4}}\mathrm{d}x=\left(\dfrac{3ax^{2}}{b^{2}}+\dfrac{9a^{2}x}{2b^{3}}+\dfrac{11a^{3}}{6b^{4}}\right)\dfrac{1}{\left(a+bx\right)^{3}}+\dfrac{1}{b^{4}}\ln\left|a+bx\right|
$$

64.
$$
\int\dfrac{x^{3}}{\left(a+bx\right)^{5}}\mathrm{d}x=-\left(\dfrac{x^{3}}{b}+\dfrac{3ax^{2}}{2b^{2}}+\dfrac{a^{2}x}{b^{3}}+\dfrac{a^{3}}{4b^{4}}\right)\dfrac{1}{\left(a+bx\right)^{4}}
$$

65.
$$
\int\dfrac{x^{m}}{a+bx}\mathrm{d}x=\dfrac{1}{b}\left(\left(-\dfrac{a}{b}\right)^{m}\ln\left|a+bx\right|+x^{m}\cdot\sum_{k=0}^{m-1}\dfrac{1}{m-k}\left(-\dfrac{a}{bx}\right)^{k}\right) 
$$

66.
$$
\int\dfrac{x^{m}}{\left(a+bx\right)^{2}}\mathrm{d}x=\sum_{k=1}^{m-1}\left(-1\right)^{k-1}\dfrac{ka^{k-1}x^{m-k}}{\left(m-k\right)b^{k+1}}+\left(-1\right)^{m-1}\dfrac{a^{m}}{b^{m+1}\left(a+bx\right)}+\left(-1\right)^{m+1}\dfrac{ma^{m-1}}{b^{m+1}}\ln\left|a+bx\right|
$$

67.
$$
\int\dfrac{x^{m}}{\left(a+bx\right)^{n}}\mathrm{d}x=\dfrac{1}{b^{m+1}}\sum_{k=0}^{m}C\left(m,n,k\right) ,C\left(m,n,k\right) =\begin{cases}\begin{pmatrix}m\\k\\\end{pmatrix}\dfrac{\left(-a\right)^{k}\left(a+bx\right)^{m-n-k+1}}{m-n-k+1},m-n-k+1\neq 0\\\begin{pmatrix}m\\n-1\\\end{pmatrix}\left(-a\right)^{m-n+1}\ln\left|a+bx\right|,m-n-k+1=0\end{cases}
$$

68.
$$
\int\dfrac{\mathrm{d}x}{x\left(a+bx\right)}=-\dfrac{1}{a}\ln\left|\dfrac{a+bx}{x}\right|
$$

69.
$$
\int\dfrac{\mathrm{d}x}{x\left(a+bx\right)^{2}}=\dfrac{1}{a\left(a+bx\right)}-\dfrac{1}{a^{2}}\ln\left|\dfrac{a+bx}{x}\right|
$$

70.
$$
\int 
$$

71.
$$
\int 
$$

72.
$$
\int 
$$

73.
$$
\int 
$$

74.
$$
\int 
$$

75.
$$
\int 
$$

76.
$$
\int 
$$

77.
$$
\int 
$$

78.
$$
\int 
$$

79.
$$
\int 
$$

80.
$$
\int 
$$

81.
$$
\int 
$$

82.
$$
\int 
$$

83.
$$
\int 
$$

84.
$$
\int 
$$

85.
$$
\int 
$$

86.
$$
\int 
$$

87.
$$
\int 
$$
